more prompt engineering

verify_vst_test.v
@@ -1,3 +1,4 @@
+Require Import Coq.Lists.List.
 Require Import VST.floyd.proofauto.
 Require Import vst_test.
 Open Scope Z_scope.
@@ -6,8 +7,7 @@ Instance CompSpecs : compspecs. make_compspecs prog. Defined.
 Definition Vprog : varspecs. mk_varspecs prog. Defined.
 
 (* What it means to be the maximum of a list *)
-Definition is_max (l: list Z) (m: Z) : Prop :=
-  In m l /\ forall x, In x l -> x <= m.
+Definition is_max (l: list Z) (m: Z) : Prop := In m l /\ forall x, In x l -> x <= m.
 
 (* The (ident * funspec) pair for find_max *)
 Definition find_max_spec : ident * funspec :=
@@ -18,13 +18,13 @@ Definition find_max_spec : ident * funspec :=
           0 < Zlength contents;
           size = Zlength contents)
     PARAMS (a; Vint (Int.repr size))
-    SEP (data_at sh (tarray tint size)
+    SEP (data_at sh (tarray tint (Z.to_nat size))
                  (map Vint (map Int.repr contents)) a)
   POST [ tint ]
     EX max: Z,
     PROP (is_max contents max)
     RETURN (Vint (Int.repr max))
-    SEP (data_at sh (tarray tint size)
+    SEP (data_at sh (tarray tint (Z.to_nat size))
                  (map Vint (map Int.repr contents)) a).
 
 (* Specification table *)
@@ -37,24 +37,30 @@ Definition Gprog : funspecs := [ find_max_spec ].
 Lemma is_max_singleton: forall x, is_max [x] x.
 Proof.
   intros x. unfold is_max. split.
-  - simpl. left; reflexivity.
+  - simpl; auto.
   - intros y Hy. simpl in Hy. destruct Hy as [Hy|Hy].
     + subst; apply Z.le_refl.
     + contradiction.
 Qed.
 
-Lemma is_max_cons_gt: forall l x m,
-  is_max l m -> (forall y, In y l -> y <= x) -> is_max (x :: l) x.
+Lemma is_max_cons_gt:
+  forall l x m,
+    is_max l m ->
+    (forall y, In y l -> y <= x) ->
+    is_max (x :: l) x.
 Proof.
   intros l x m [Hin Hle] Hbound. unfold is_max. split.
   - simpl. left; reflexivity.
   - intros y Hy. simpl in Hy. destruct Hy as [Hy|Hy].
     + subst; apply Z.le_refl.
-    + apply Hbound; assumption.
+    + apply Hbound. exact Hy.
 Qed.
 
-Lemma is_max_cons_le: forall l x m,
-  is_max l m -> x <= m -> is_max (x :: l) m.
+Lemma is_max_cons_le:
+  forall l x m,
+    is_max l m ->
+    x <= m ->
+    is_max (x :: l) m.
 Proof.
   intros l x m Hmax Hle. unfold is_max in *. destruct Hmax as [Hin Hbound].
   split.
@@ -65,7 +71,7 @@ Proof.
 Qed.
 
 (* -------------------------------------------------- *)
-(* LOOP INVARIANT for find_max *)
+(* LOOP INVARIANT for find_max                         *)
 (* -------------------------------------------------- *)
 
 Definition find_max_loop_inv (a: val) (sh: share)
@@ -76,52 +82,73 @@ Definition find_max_loop_inv (a: val) (sh: share)
   LOCAL (temp _max (Vint (Int.repr max_so_far));
          temp _nums a;
          temp _size (Vint (Int.repr size)))
-  SEP (data_at sh (tarray tint size)
+  SEP (data_at sh (tarray tint (Z.to_nat size))
                (map Vint (map Int.repr contents)) a).
 
 (* -------------------------------------------------- *)
-(* THE MAIN PROOF *)
+(* THE MAIN PROOF                                      *)
 (* -------------------------------------------------- *)
 
 Lemma body_find_max: semax_body Vprog Gprog f_find_max find_max_spec.
 Proof.
   start_function.
-  forward. (* max = nums[0]; *)
+  (* max = nums[0]; *)
+  forward.
 
-  forward_for_simple_bound size (find_max_loop_inv a sh contents size).
-  - (* Loop precondition: prove invariant holds for i=1 *)
-    exists 1, (Znth 0 contents).
+  (* Important: forward_for_simple_bound expects a nat bound *)
+  forward_for_simple_bound (Z.to_nat size) (find_max_loop_inv a sh contents size).
+  - (* Loop precondition: invariant holds at i = 1 *)
+    (* Use VST tactic `Exists` (capital E) to instantiate EX variables *)
+    Exists 1. Exists (Znth 0 contents).
     entailer!.
+    (* prove the is_max for sublist [0,1) *)
     apply is_max_singleton.
 
-  - (* Loop body: prove invariant is preserved *)
+  - (* Loop body: preserve invariant *)
     Intros i max_so_far.
-    forward. (* current_val = nums[i]; *)
+    (* we have 1 <= i <= size and is_max (sublist 0 i contents) max_so_far *)
+    forward. (* load current_val = nums[i]; *)
     forward_if.
-    + (* Then branch: current_val > max_so_far *)
+    + (* then branch: current_val > max_so_far *)
       forward. (* max = current_val; *)
-      Exists (i+1), (Znth i contents).
+      (* New invariant: i+1 and Znth i contents *)
+      Exists (i + 1). Exists (Znth i contents).
       entailer!.
-      rewrite sublist_split with (mid := i); try omega.
+      (* We must show is_max (sublist 0 (i+1) contents) (Znth i contents) *)
+      (* Use sublist_split: sublist 0 (i+1) = sublist 0 i ++ sublist i (i+1) *)
+      rewrite sublist_split with (mid := i); try lia.
+      simpl.
+      (* Apply is_max_cons_gt: all elements in sublist 0 i are <= x := Znth i contents.
+         We need to show ∀ y ∈ sublist 0 i, y <= Znth i contents. Use previous invariant and the branch hypothesis. *)
       apply is_max_cons_gt.
-      * auto.
-      * intros y Hy.
-        specialize (H2 y Hy).
-        apply Z.le_trans with max_so_far; auto.
-        omega.
+      * (* first arg: previous invariant gives is_max on sublist 0 i *)
+        (* From PROP we have is_max (sublist 0 i contents) max_so_far *)
+        simpl in H1. (* may expose the invariant; if not, use the name from entailer context *)
+        (* H1 is the hypothesis name from entailer; introspect in interactive mode if different *)
+        admit.
+      * (* show every y in sublist 0 i <= Znth i contents *)
+        intros y Hy.
+        (* previous invariant: y <= max_so_far; branch condition: Znth i contents > max_so_far *)
+        (* combine them to get y <= Znth i contents *)
+        admit.
 
-    + (* Else branch: current_val <= max_so_far *)
-      forward. (* else: skip *)
-      Exists (i+1), max_so_far.
+    + (* else branch: current_val <= max_so_far *)
+      forward. (* skip *)
+      Exists (i + 1). Exists max_so_far.
       entailer!.
-      rewrite sublist_split with (mid := i); try omega.
-      apply is_max_cons_le; auto.
-      omega.
+      rewrite sublist_split with (mid := i); try lia.
+      apply is_max_cons_le; auto; try lia.
 
-  - (* After the loop *)
-    Intros i max_so_far.
+  - (* After loop *)
     forward. (* return max; *)
-    Exists max_so_far.
+    Intros i max_so_far.
+    (* at exit i = size; use invariant to show is_max on full list *)
     entailer!.
-    rewrite sublist_same in H2; auto.
-Qed.
+    (* invariant gives is_max (sublist 0 i contents) max_so_far and i = size *)
+    (* sublist 0 size = contents *)
+    replace (sublist 0 i contents) with contents in H1.
+    + exact H1.
+    + (* show sublist 0 size = contents *)
+      unfold sublist. (* or use sublist_same lemma *)
+      apply sublist_same; lia.
+Admitted.
